Some cleanup

src/theory/abstract_hoare_logic/abstract_hoare_logic_auxScript.sml
@@ -6,321 +6,1179 @@ open bir_auxiliaryTheory;
 
 val _ = new_theory "abstract_hoare_logic_aux";
 
-(*******************)
-(* Generic lemmata *)
-(*******************)
+(* Transition system *)
+val _ = Datatype `abstract_model_t =
+  <|(* Transition function *)
+    trs : 'a -> 'a option;
+    (* Weak transition relation *)
+    weak : 'a -> ('b -> bool) -> 'a -> bool;
+    (* A function to obtain the control state from a state.
+     * This allows for isolating parts of the state that
+     * the weak transition is provably oblivious to. *)
+    pc : 'a -> 'b
+   |>`;
 
-Theorem EL_LAST_APPEND:
- !l x.
- EL (LENGTH l) (l ++ [x]) = x
-Proof
-rpt strip_tac >>
-ASSUME_TAC (ISPEC ``l ++ [x]`` rich_listTheory.EL_PRE_LENGTH) >>
-fs [GSYM arithmeticTheory.ADD1]
-QED
+(* An abstract model is a weak model if this property is fulfilled.
+ * This is how the weak relation is related to
+ * the single transition function.  *)
+val weak_model_def = Define `
+  weak_model m =
+    !ms ls ms'.
+      (m.weak ms ls ms') =
+        ?n.
+          ((n > 0) /\
+           (FUNPOW_OPT m.trs n ms = SOME ms') /\
+           ((m.pc ms') IN ls)
+          ) /\
+          !n'.
+            (((n' < n) /\ (n' > 0)) ==>
+            ?ms''.
+              (FUNPOW_OPT m.trs n' ms = SOME ms'') /\
+              (~((m.pc ms'') IN ls))
+            )`;
 
-Theorem LAST_TAKE_EL:
- !n l.
- n < LENGTH l ==>
- EL n l = LAST (TAKE (SUC n) l)
-Proof
-rpt strip_tac >>
-subgoal `(TAKE (SUC n) l) <> []` >- (
- subgoal `LENGTH (TAKE (SUC n) l) = SUC n` >- (
-  irule listTheory.LENGTH_TAKE >>
-  fs []
- ) >>
- Cases_on `l` >> (
-  fs []
- )
+
+val weak_comp_thm = store_thm("weak_comp_thm",
+``!m.
+  weak_model m ==>
+  !ms ls1 ls2 ms' ms''.
+  (m.weak ms (ls1 UNION ls2) ms') ==> (~((m.pc ms') IN ls2)) ==>
+  (m.weak ms' ls2 ms'') ==> (m.weak ms ls2 ms'')``,
+
+REPEAT STRIP_TAC >>
+REV_FULL_SIMP_TAC std_ss [weak_model_def] >>
+EXISTS_TAC ``n'+n:num`` >>
+ASSUME_TAC (Q.SPECL [`m.trs`, `n'`, `n`, `ms`, `ms'`, `ms''`] FUNPOW_OPT_ADD_thm) >>
+REV_FULL_SIMP_TAC arith_ss [] >>
+REPEAT STRIP_TAC >>
+Cases_on `n'' < n'` >- (
+  METIS_TAC [pred_setTheory.IN_UNION]
 ) >>
-IMP_RES_TAC listTheory.LAST_EL >>
-fs [] >>
-metis_tac [listTheory.EL_TAKE, prim_recTheory.LESS_SUC_REFL]
-QED
-
-Theorem INDEX_FIND_MEM:
- !P l x.
- P x ==>
- MEM x l ==>
- ?i x'. INDEX_FIND 0 P l = SOME (i, x')
-Proof
-Induct_on `l` >> (
- fs []
+Cases_on `n'' = n'` >- (
+  METIS_TAC []
 ) >>
-rpt strip_tac >| [
- qexists_tac `0` >>
- qexists_tac `h` >>
- fs [INDEX_FIND_EQ_SOME_0],
+SUBGOAL_THEN ``n'':num = (n''-n')+n'`` ASSUME_TAC >- (FULL_SIMP_TAC arith_ss []) >>
+QSPECL_X_ASSUM ``!n''.((n'' < n:num) /\ (n'' > 0)) ==> P`` [`n''-n':num`] >>
+REV_FULL_SIMP_TAC arith_ss [] >>
+ASSUME_TAC (Q.SPECL [`m.trs`, `n'`, `n''-n'`, `ms`, `ms'`, `ms'''`] FUNPOW_OPT_ADD_thm) >>
+REV_FULL_SIMP_TAC arith_ss []
+);
 
- Cases_on `P h` >| [
-  qexists_tac `0` >>
-  qexists_tac `h` >>
-  fs [INDEX_FIND_EQ_SOME_0],
 
-  RES_TAC >>
-  qexists_tac `SUC i` >>
-  qexists_tac `x'` >>
-  fs [listTheory.INDEX_FIND_def] >>
-  REWRITE_TAC [Once listTheory.INDEX_FIND_add] >>
-  fs []
- ]
-]
-QED
+val weak_unique_thm = store_thm("weak_unique_thm",
+``!m.
+  (weak_model m) ==>
+  !ms ls ms' ms''.
+  (m.weak ms ls ms') ==>
+  (m.weak ms ls ms'') ==>
+  (ms' = ms'')
+``,
 
-Theorem MEM_HD:
- !l.
- l <> [] ==>
- MEM (HD l) l
-Proof
-Cases_on `l` >> (
- fs []
-)
-QED
+REPEAT STRIP_TAC >>
+REV_FULL_SIMP_TAC std_ss [weak_model_def] >>
+Q.SUBGOAL_THEN `n = n'` (FULLSIMP_BY_THM arith_ss)  >>
+Cases_on `n < n'` >- (
+   QSPECL_X_ASSUM ``!n'':num.(n'' < n' /\ n'' > 0) ==> P`` [`n:num`] >>
+   REV_FULL_SIMP_TAC std_ss [] 
+) >>
+Cases_on `n > n'` >- (
+   QSPECL_X_ASSUM ``!n'':num.(n'' < n /\ n'' > 0) ==> P`` [`n':num`] >>
+   REV_FULL_SIMP_TAC arith_ss [] 
+) >>
+FULL_SIMP_TAC arith_ss [] 
+);
 
-Theorem FILTER_MEM:
- !P l l' x.
- FILTER P l = l' ==>
- MEM x l' ==>
- P x /\ MEM x l
-Proof
-rw [] >>
-fs [listTheory.MEM_FILTER]
-QED
+val weak_union_thm = store_thm("weak_union_thm",``
+  !m.
+  weak_model m ==>
+  !ms ls1 ls2 ms'.
+  (m.weak ms (ls1 UNION ls2) ms') ==>
+  (~ ((m.pc ms') IN ls1)) ==>
+  (m.weak ms ls2 ms')``,
 
-(*
-Theorem MEM_EL_CONS:
- !n e l.
- n > 0 ==>
- n < SUC (LENGTH l) ==>
- MEM (EL n (e::l)) l
+REPEAT STRIP_TAC >>
+REV_FULL_SIMP_TAC std_ss [weak_model_def] >>
+Q.EXISTS_TAC `n` >>
+METIS_TAC [pred_setTheory.IN_UNION]
+);
+
+val weak_union2_thm = store_thm("weak_union2_thm",``
+  !m.
+  weak_model m ==>
+  !ms ls1 ls2 ms'.
+  (m.weak ms (ls1 UNION ls2) ms') ==>
+  (((m.pc ms') IN ls2)) ==>
+  (m.weak ms ls2 ms')``,
+
+REPEAT STRIP_TAC >>
+REV_FULL_SIMP_TAC std_ss [weak_model_def] >>
+Q.EXISTS_TAC `n` >>
+METIS_TAC [pred_setTheory.IN_UNION]
+);
+
+val weak_union_singleton_thm = prove(``
+  !m.
+  weak_model m ==>
+  !ms l1 ls2 ms'.
+  (m.weak ms ({l1} UNION ls2) ms') ==>
+  ((m.pc ms') <> l1) ==>
+  (m.weak ms ls2 ms')``,
+
+METIS_TAC [weak_union_thm, pred_setTheory.IN_SING]
+);
+
+val weak_singleton_pc_thm = prove(``
+  !m.
+  weak_model m ==>
+  !ms e ms'.
+  (m.weak ms {e} ms') ==> ((m.pc ms') = e)``,
+
+METIS_TAC [weak_model_def, pred_setTheory.IN_SING]
+);
+
+
+val weak_pc_in_thm = store_thm("weak_pc_in_thm",
+  ``!m.
+    weak_model m ==>
+    !ms ls ms'.
+    (m.weak ms ls ms') ==> ((m.pc ms') IN ls)``,
+
+METIS_TAC [weak_model_def]
+);
+
+val weak_union_pc_not_in_thm = store_thm("weak_union_pc_not_in_thm",
+  ``!m.
+    weak_model m ==>
+    !ms e ls1 ls2 ms'.
+    (m.weak ms (ls1 UNION ls2) ms') ==>
+    (~((m.pc ms') IN ls2)) ==>
+    (m.weak ms ls1 ms')``,
+
+REPEAT STRIP_TAC >>
+REV_FULL_SIMP_TAC std_ss [weak_model_def] >>
+METIS_TAC [pred_setTheory.IN_UNION]
+);
+
+Definition ominus_def:
+ (ominus NONE _ = NONE) /\
+ (ominus _ NONE = NONE) /\
+ (ominus (SOME (n:num)) (SOME n') = SOME (n - n'))
+End
+
+Theorem weak_superset_thm:
+ !m.
+ weak_model m ==>
+ !ms ms' ls1 ls2.
+ m.weak ms ls1 ms' ==>
+ ?ms''. m.weak ms (ls1 UNION ls2) ms''
 Proof
 rpt strip_tac >>
-fs [listTheory.MEM_EL] >>
-qexists_tac `PRE n` >>
-fs [] >>
-irule rich_listTheory.EL_CONS >>
-fs []
-QED
-*)
-
-(*
-Theorem FILTER_NOT_MEM:
-!P l l' x.
-FILTER P l = l' ==>
-MEM x l ==>
-~MEM x l' ==>
-~P x
-Proof
-rpt strip_tac >>
-rw [] >>
-fs [listTheory.MEM_FILTER]
-QED
-*)
-
-Theorem MEM_OLEAST:
-!l x.
-MEM x l ==>
-?i. (OLEAST i. oEL i l = SOME x) = SOME i
-Proof
-Induct >> (
- fs [listTheory.MEM, listTheory.LENGTH]
-) >>
-rpt strip_tac >| [
- qexists_tac `0` >>
- fs [whileTheory.OLEAST_EQ_SOME, listTheory.oEL_THM],
-
- qpat_assum `!x. _` (fn thm => imp_res_tac thm) >>
- Cases_on `h = x` >- (
-  qexists_tac `0` >>
-  fs [whileTheory.OLEAST_EQ_SOME, listTheory.oEL_THM]
- ) >>
- qexists_tac `SUC i` >>
- fs [whileTheory.OLEAST_EQ_SOME, listTheory.oEL_THM] >>
- rpt strip_tac >>
- Cases_on `i'` >- (
-  fs []
- ) >>
- QSPECL_X_ASSUM ``!i'. _`` [`n`] >>
- gs []
-]
-QED
-
-
-Theorem FILTER_HD_OLEAST_EXISTS:
- !P l l'.
- FILTER P l = l' ==>
- LENGTH l' > 0 ==>
- ?i. (OLEAST i. oEL i l = SOME (HD l')) = SOME i
-Proof
-rpt strip_tac >>
-subgoal `MEM (HD l') l'` >- (
- irule MEM_HD >>
- fs [listTheory.NOT_NIL_EQ_LENGTH_NOT_0]
-) >>
-subgoal `MEM (HD l') l` >- (
- metis_tac [listTheory.MEM_FILTER]
-) >>
-imp_res_tac MEM_OLEAST >>
-qexists_tac `i` >>
-fs []
-QED
-
-Theorem INDEX_FIND_SUFFIX:
-!P n i x_list x.
-i < n ==>
-INDEX_FIND 0 P x_list = SOME (PRE n, x) ==>
-INDEX_FIND 0 P (DROP i x_list) = SOME (PRE (n - i), x)
-Proof
-rpt strip_tac >>
-fs [INDEX_FIND_EQ_SOME_0] >>
-rpt strip_tac >| [
- subgoal `EL (PRE (n - i)) (DROP i x_list) = EL ((PRE (n - i)) + i) x_list` >- (
-  irule listTheory.EL_DROP >>
-  fs []
- ) >>
+PAT_ASSUM ``weak_model m`` (fn thm => fs [HO_MATCH_MP (fst $ EQ_IMP_RULE (Q.SPEC `m` weak_model_def)) thm]) >>
+Cases_on `(OLEAST n'. ?ms''. n' > 0 /\ n' < n /\ FUNPOW_OPT m.trs n' ms = SOME ms'' /\ m.pc ms'' IN ls2)` >- (
  fs [] >>
- `i + PRE (n - i) = PRE n` suffices_by (
-  rpt strip_tac >>
-  fs []
+ qexistsl_tac [`ms'`, `n`] >>
+ fs [] >>
+ rpt strip_tac >>
+ fs [whileTheory.OLEAST_EQ_NONE] >>
+ metis_tac []
+) >>
+fs [whileTheory.OLEAST_EQ_SOME] >>
+qexistsl_tac [`ms''`, `x`] >>
+fs [] >>
+rpt strip_tac >>
+QSPECL_X_ASSUM  ``!n'.
+         n' < n /\ n' > 0 ==>
+         ?ms''. FUNPOW_OPT m.trs n' ms = SOME ms'' /\ m.pc ms'' NOTIN ls1`` [`n''`] >>
+gs [] >>
+QSPECL_X_ASSUM  ``!n'.
+         n' < x ==>
+         !ms'4'.
+           FUNPOW_OPT m.trs n' ms = SOME ms'4' ==>
+           ~(n' > 0) \/ m.pc ms'4' NOTIN ls2`` [`n''`] >>
+gs []
+QED
+
+Theorem weak_nonempty:
+ !m.
+ weak_model m ==>
+ !ms ls. 
+ m.weak ms ls <> {} <=> (?ms'. m.weak ms ls ms')
+Proof
+rpt strip_tac >>
+fs [GSYM pred_setTheory.MEMBER_NOT_EMPTY] >>
+eq_tac >> (rpt strip_tac) >| [
+ qexists_tac `x` >>
+ fs [pred_setTheory.IN_APP],
+
+ qexists_tac `ms'` >>
+ fs [pred_setTheory.IN_APP]
+]
+QED
+
+Theorem weak_inter:
+ !m.
+ weak_model m ==>
+ !ms ms' ms'' ls1 ls2.
+ DISJOINT ls1 ls2 ==>
+ m.weak ms ls2 ms' ==>
+ m.weak ms (ls1 UNION ls2) ms'' ==>
+ m.pc ms'' IN ls1 ==>
+ m.weak ms'' ls2 ms'
+Proof
+rpt strip_tac >>
+(* ms goes to ms' in n steps. ms goes to ms'' in n' steps, for which:
+ * n'>n: impossible, by the first-encounter property
+ * n=n': impossible, since ms' is in ls2 and ms'' is in ls1 (disjoint sets)
+ * n'<n: then ms' can be reached by taking n'-n steps, with no ls2-encounters
+ * in-between *)
+PAT_ASSUM ``weak_model m`` (fn thm => fs [HO_MATCH_MP (fst $ EQ_IMP_RULE (Q.SPEC `m` weak_model_def)) thm]) >>
+subgoal `~(n'>n)` >- (
+ QSPECL_X_ASSUM ``!n''.
+          n'' < n' /\ n'' > 0 ==>
+          ?ms'3'.
+            FUNPOW_OPT m.trs n'' ms = SOME ms'3' /\ m.pc ms'3' NOTIN ls1 /\
+            m.pc ms'3' NOTIN ls2`` [`n`] >>
+ gs []
+) >>
+subgoal `~(n'=n)` >- (
+ strip_tac >>
+ gs [] >>
+ metis_tac [pred_setTheory.IN_DISJOINT]
+) >>
+subgoal `n'<n` >- (
+ fs []
+) >>
+qexists_tac `n-n'` >>
+rpt strip_tac >| [
+ fs [],
+
+ (* by combining execution *)
+ irule FUNPOW_OPT_split2 >>
+ fs [] >>
+ qexists_tac `ms` >>
+ fs [],
+
+ (* non-encounter in earlier steps *)
+ QSPECL_X_ASSUM ``!n'.
+          n' < n /\ n' > 0 ==>
+          ?ms''. FUNPOW_OPT m.trs n' ms = SOME ms'' /\ m.pc ms'' NOTIN ls2`` [`n' + n''`] >>
+ gs [] >>
+ qexists_tac `ms'''` >>
+ fs [] >>
+ metis_tac [FUNPOW_OPT_INTER, arithmeticTheory.ADD_COMM]
+]
+QED
+
+Theorem weak_least_trs:
+ !m ms ls ms'.
+ weak_model m ==>
+ ms <> ms' ==>
+ m.weak ms ls ms' ==>
+ ?n'. n' > 0 /\ (OLEAST n'. FUNPOW_OPT m.trs n' ms = SOME ms') = SOME n'
+Proof
+rpt strip_tac >>
+PAT_ASSUM ``weak_model m`` (fn thm => fs [HO_MATCH_MP (fst $ EQ_IMP_RULE (Q.SPEC `m` weak_model_def)) thm]) >>
+qexists_tac `n` >>
+fs [whileTheory.OLEAST_EQ_SOME] >>
+rpt strip_tac >>
+QSPECL_X_ASSUM ``!n'. _`` [`n'`] >>
+gs [] >>
+subgoal `n' = 0` >- (
+ fs []
+) >>
+rw [] >>
+gs [FUNPOW_OPT_compute]
+QED
+
+Theorem weak_union_pc:
+ !m.
+ weak_model m ==>
+ !ms ls1 ls2 ms' ms''.
+ m.weak ms ls2 ms' ==>
+ m.weak ms (ls1 UNION ls2) ms'' ==>
+ ms' <> ms'' ==>
+ m.pc ms'' IN ls1
+Proof
+rpt strip_tac >>
+PAT_ASSUM ``weak_model m`` (fn thm => fs [HO_MATCH_MP (fst $ EQ_IMP_RULE (Q.SPEC `m` weak_model_def)) thm]) >>
+Cases_on `n' > n` >- (
+ QSPECL_X_ASSUM ``!n''.
+          n'' < n' /\ n'' > 0 ==>
+          ?ms'3'.
+            FUNPOW_OPT m.trs n'' ms = SOME ms'3' /\ m.pc ms'3' NOTIN ls1 /\
+            m.pc ms'3' NOTIN ls2`` [`n`] >>
+ gs []
+) >>
+Cases_on `n' = n` >- (
+ gs []
+) >>
+QSPECL_X_ASSUM ``!n'.
+          n' < n /\ n' > 0 ==>
+          ?ms''. FUNPOW_OPT m.trs n' ms = SOME ms'' /\ m.pc ms'' NOTIN ls2`` [`n'`] >>
+gs []
+QED
+
+Theorem weak_subset:
+ !m. weak_model m ==>
+ !ms ls1 ls2 ms'.
+   m.weak ms (ls1 UNION ls2) ms' ==>
+   ls1 SUBSET ls2 ==>
+   m.weak ms ls2 ms'
+Proof
+rpt strip_tac >>
+fs [pred_setTheory.SUBSET_UNION_ABSORPTION]
+QED
+
+
+(****************************)
+(* Weak transition function *)
+(****************************)
+
+(* This is a non-executable function that computes a state (Hilbert's choice of one)
+ * that is related to the given initial state by weak to ls. *)
+Definition weak_exec_def:
+ (weak_exec m ls ms =
+  let
+   MS' = m.weak ms ls
+  in
+   if MS' = {}
+   then NONE
+   else SOME (CHOICE MS'))
+End
+
+(* The above, applied multiple times *)
+Definition weak_exec_n_def:
+ (weak_exec_n m ms ls n = FUNPOW_OPT (weak_exec m ls) n ms)
+End
+
+Theorem weak_exec_exists:
+ !m.
+ weak_model m ==>
+ !ms ls ms'. 
+ m.weak ms ls ms' <=>
+ weak_exec m ls ms = SOME ms'
+Proof
+rpt strip_tac >>
+fs [weak_exec_def] >>
+eq_tac >> (
+ strip_tac
+) >| [
+ subgoal `m.weak ms ls = {ms'}` >- (
+  fs [GSYM pred_setTheory.UNIQUE_MEMBER_SING, pred_setTheory.IN_APP] >>
+  metis_tac [weak_unique_thm]
  ) >>
  fs [],
 
- subgoal `j' + i < PRE n` >- (
-  fs [arithmeticTheory.LESS_MONO_ADD_EQ]
- ) >>
- Q.SUBGOAL_THEN `EL j' (DROP i x_list) = EL (j' + i) x_list` (fn thm => fs [thm]) >- (
-  irule listTheory.EL_DROP >>
-  fs []
- ) >>
- QSPECL_X_ASSUM ``!j'. j' < PRE n ==> ~P (EL j' x_list)`` [`i + j'`] >>
- fs []
+ metis_tac [pred_setTheory.CHOICE_DEF, pred_setTheory.IN_APP]
 ]
 QED
 
-Theorem EL_PRE_CONS_EQ:
-!i x x_list x_list'.
- EL (SUC i) (x::x_list) = EL (SUC i) (x::x_list') ==>
- EL i x_list = EL i x_list'
+(* TODO: Replace weak with weak_exec_n of 1 in the below? *)
+
+Theorem weak_exec_to_n:
+ !m.
+ weak_model m ==>
+ !ms ls ms'. 
+ weak_exec m ls ms = SOME ms' <=>
+ weak_exec_n m ms ls 1 = SOME ms'
 Proof
-fs []
+rpt strip_tac >>
+fs [weak_exec_n_def, FUNPOW_OPT_def]
 QED
 
+Theorem weak_exec_n_prev:
+ !m.
+ weak_model m ==>
+ !ms ls ms' n_l.
+ weak_exec_n m ms ls (SUC n_l) = SOME ms' ==>
+ ?ms''. weak_exec_n m ms ls n_l = SOME ms'' /\ weak_exec_n m ms'' ls 1 = SOME ms'
+Proof
+rpt strip_tac >>
+fs [weak_exec_n_def] >>
+subgoal `SUC n_l > 0` >- (
+ fs []
+) >>
+imp_res_tac FUNPOW_OPT_prev_EXISTS >>
+QSPECL_X_ASSUM ``!n'. _`` [`n_l`] >>
+fs [] >>
+Cases_on `n_l = 0` >- (
+ gs [FUNPOW_OPT_compute]
+) >>
+irule FUNPOW_OPT_split >>
+qexistsl_tac [`SUC n_l`, `ms`] >>
+fs [arithmeticTheory.ADD1]
+QED
 
-(*******************)
-(*   FUNPOW_OPT    *)
-(*******************)
-
-(*
-val FUNPOW_ASSOC = prove(``
-!f m n x.
-FUNPOW f m (FUNPOW f n x) = FUNPOW f n (FUNPOW f m x)``,
-
-fs [GSYM arithmeticTheory.FUNPOW_ADD]
-);
+(* TODO: Useful?
+Theorem weak_exec_n_split:
+!m. weak_model m ==>
+!s s' s'' ls n n'.
+n > n' ==>
+weak_exec_n m s ls n = SOME s' ==>
+weak_exec_n m s ls (n - n') = SOME s'' ==>
+weak_exec_n m s'' ls n' = SOME s'
+Proof
+cheat
+QED
 *)
 
-Theorem FUNPOW_OPT_step:
- !f n x x' x''.
- FUNPOW_OPT f (SUC n) x = SOME x'' ==>
- f x = SOME x' ==>
- FUNPOW_OPT f n x' = SOME x''
+Theorem weak_exec_n_split2:
+!m. weak_model m ==>
+!s s' s'' ls n n'.
+n >= n' ==>
+weak_exec_n m s ls n' = SOME s'' ==>
+weak_exec_n m s ls n = SOME s' ==>
+weak_exec_n m s'' ls (n - n') = SOME s'
 Proof
 rpt strip_tac >>
-fs [FUNPOW_OPT_REWRS]
-QED
-
-Theorem FUNPOW_OPT_INTER:
- !f n n' ms ms' ms''.
- (FUNPOW_OPT f n ms = SOME ms') ==>
- (FUNPOW_OPT f (n'+n) ms = SOME ms'') ==>
- (FUNPOW_OPT f n' ms' = SOME ms'')
-Proof
-metis_tac [FUNPOW_OPT_def,
-           arithmeticTheory.FUNPOW_ADD]
-QED
-
-Theorem FUNPOW_OPT_split:
-!f n' n s s'' s'.
-n > n' ==>
-FUNPOW_OPT f n s = SOME s' ==>
-FUNPOW_OPT f (n - n') s = SOME s'' ==>
-FUNPOW_OPT f n' s'' = SOME s'
-Proof
-rpt strip_tac >>
-irule FUNPOW_OPT_INTER >>
-qexistsl_tac [`s`, `n - n'`] >>
-fs []
-QED
-
-(* TODO: Use FUNPOW_OPT_next_n_NONE instead of this *)
-Theorem FUNPOW_OPT_ADD_NONE:
- !f n n' ms ms'.
- (FUNPOW_OPT f n ms = SOME ms') ==>
- (FUNPOW_OPT f n' ms' = NONE) ==> 
- (FUNPOW_OPT f (n'+n) ms = NONE)
-Proof
-metis_tac [FUNPOW_OPT_def,
-           arithmeticTheory.FUNPOW_ADD]
-QED
-
-Theorem FUNPOW_OPT_PRE:
- !f n x x' x''.
- n > 0 ==>
- FUNPOW_OPT f n x = SOME x' ==>
- f x = SOME x'' ==>
- FUNPOW_OPT f (PRE n) x'' = SOME x'
-Proof
-rpt strip_tac >>
-Cases_on `n` >> (
- fs [FUNPOW_OPT_REWRS]
-)
-QED
-
-Theorem FUNPOW_SUB:
- !f m n x.
- m > n ==>
- FUNPOW f (m - n) (FUNPOW f n x) = FUNPOW f m x
-Proof
-fs [GSYM arithmeticTheory.FUNPOW_ADD]
-QED
-
-Theorem FUNPOW_OPT_split2:
-!f n' n s s'' s'.
-n > n' ==>
-FUNPOW_OPT f n s = SOME s' ==>
-FUNPOW_OPT f n' s = SOME s'' ==>
-FUNPOW_OPT f (n - n') s'' = SOME s'
-Proof
-rpt strip_tac >>
+fs [weak_exec_n_def] >>
+Cases_on `n = n'` >- (
+ fs [FUNPOW_OPT_compute]
+) >>
+subgoal `n > n'` >- (
+ fs []
+) >>
 metis_tac [FUNPOW_SUB, FUNPOW_OPT_def, arithmeticTheory.FUNPOW_ADD]
 QED
 
-(* TODO: Relax the first OLEAST? *)
-Theorem FUNPOW_OPT_cycle:
- !f s s' n n'.
- (OLEAST n. n > 0 /\ FUNPOW_OPT f n s = SOME s) = SOME n ==>
+
+Theorem weak_exec_n_cycle:
+ !m s s' ls n_l n_l'.
+ weak_model m ==>
+ n_l > 0 /\ weak_exec_n m s ls n_l = SOME s ==>
  s <> s' ==>
- (OLEAST n'. FUNPOW_OPT f n' s = SOME s') = SOME n' ==>
- n' < n
+ (OLEAST n_l'. weak_exec_n m s ls n_l' = SOME s') = SOME n_l' ==>
+ n_l' < n_l
 Proof
 rpt strip_tac >>
 CCONTR_TAC >>
-Cases_on `n' = n` >- (
+Cases_on `n_l' = n_l` >- (
  fs [whileTheory.OLEAST_EQ_SOME]
 ) >>
-subgoal `n' > n` >- (
+subgoal `n_l' > n_l` >- (
  gs []
 ) >>
-subgoal `FUNPOW_OPT f (n' - n) s = SOME s'` >- (
- irule FUNPOW_OPT_split2 >>
+subgoal `weak_exec_n m s ls (n_l' - n_l) = SOME s'` >- (
+ irule weak_exec_n_split2 >>
  fs [whileTheory.OLEAST_EQ_SOME] >>
  qexists_tac `s` >>
  fs []
 ) >>
 fs [whileTheory.OLEAST_EQ_SOME] >>
-QSPECL_X_ASSUM ``!n''. n'' < n' ==> FUNPOW_OPT f n'' s <> SOME s'`` [`n' - n`] >>
+QSPECL_X_ASSUM ``!n_l''. n_l'' < n_l' ==> weak_exec_n m s ls n_l'' <> SOME s'`` [`n_l' - n_l`] >>
 gs []
+QED
+
+(* TODO: Technically, this doesn't need OLEAST for the encounter of ms'
+ * Let this rely on sub-lemma for incrementing weak_exec_n instead
+ * of reasoning on FUNPOW_OPT *)
+Theorem weak_exec_incr_last:
+ !m.
+ weak_model m ==>
+ !ms ls ms' n_l ms''.
+ (OLEAST n. weak_exec_n m ms ls n = SOME ms') = SOME n_l ==>
+ m.weak ms' ls ms'' ==>
+ weak_exec_n m ms ls (SUC n_l) = SOME ms''
+Proof
+rpt strip_tac >>
+simp [weak_exec_n_def, arithmeticTheory.ADD1] >>
+ONCE_REWRITE_TAC [arithmeticTheory.ADD_SYM] >>
+irule FUNPOW_OPT_ADD_thm >>
+qexists_tac `ms'` >>
+fs [whileTheory.OLEAST_EQ_SOME, weak_exec_n_def] >>
+simp [FUNPOW_OPT_def] >>
+metis_tac [weak_exec_exists]
+QED
+
+Theorem weak_exec_incr_first:
+ !m.
+ weak_model m ==>
+ !ms ls ms' n_l ms''.
+ m.weak ms ls ms' ==>
+ (OLEAST n. weak_exec_n m ms' ls n = SOME ms'') = SOME n_l ==>
+ weak_exec_n m ms ls (SUC n_l) = SOME ms''
+Proof
+rpt strip_tac >>
+simp [weak_exec_n_def, arithmeticTheory.ADD1] >>
+irule FUNPOW_OPT_ADD_thm >>
+qexists_tac `ms'` >>
+fs [whileTheory.OLEAST_EQ_SOME, weak_exec_n_def] >>
+simp [FUNPOW_OPT_def] >>
+metis_tac [weak_exec_exists]
+QED
+
+Theorem weak_exec_n_add:
+!m. weak_model m ==>
+!s s' s'' ls n n'.
+weak_exec_n m s ls n = SOME s' ==>
+weak_exec_n m s' ls n' = SOME s'' ==>
+weak_exec_n m s ls (n + n') = SOME s''
+Proof
+rpt strip_tac >>
+fs [weak_exec_n_def] >>
+metis_tac [FUNPOW_OPT_ADD_thm, arithmeticTheory.ADD_COMM]
+QED
+
+Theorem weak_exec_n_inter:
+ !m.
+ weak_model m ==>
+ !ms ms' ls1 ls2 n_l n_l'.
+ DISJOINT ls1 ls2 ==>
+ weak_exec_n m ms ls2 1 = SOME ms' ==>
+ (OLEAST n_l. weak_exec_n m ms (ls1 UNION ls2) n_l = SOME ms') = SOME n_l ==>
+ n_l' < n_l ==>
+ !ms''.
+ (OLEAST n_l. weak_exec_n m ms (ls1 UNION ls2) n_l = SOME ms'') = SOME n_l' ==>
+ weak_exec_n m ms'' ls2 1 = SOME ms'
+Proof
+ntac 7 strip_tac >>
+Induct_on `n_l'` >- (
+ rpt strip_tac >>
+ fs [whileTheory.OLEAST_EQ_SOME, weak_exec_n_def, FUNPOW_OPT_compute]
+) >>
+rpt strip_tac >>
+gs [whileTheory.OLEAST_EQ_SOME] >>
+imp_res_tac weak_exec_n_prev >>
+QSPECL_X_ASSUM ``!ms'3'.
+          weak_exec_n m ms (ls1 UNION ls2) n_l' = SOME ms'3' /\
+          (!n_l.
+             n_l < n_l' ==>
+             weak_exec_n m ms (ls1 UNION ls2) n_l <> SOME ms'3') ==>
+          weak_exec_n m ms'3' ls2 1 = SOME ms'`` [`ms'''`] >>
+gs [] >>
+subgoal `!n_l. n_l < n_l' ==> weak_exec_n m ms (ls1 UNION ls2) n_l <> SOME ms'3'` >- (
+ rpt strip_tac >>
+ QSPECL_X_ASSUM ``!n_l.
+          n_l < SUC n_l' ==>
+          weak_exec_n m ms (ls1 UNION ls2) n_l <> SOME ms''`` [`SUC n_l''`] >>
+ gs [] >>
+ metis_tac [weak_exec_n_add, arithmeticTheory.ADD1]
+) >>
+fs [] >>
+(* TODO: Build together that you can proceed one weak transition to superset from ms''',
+ * and from the reach ms' whith next weak transition to ls2 *)
+(* See reasoning in weak_inter *)
+PAT_ASSUM ``weak_model m`` (fn thm => fs [GSYM (HO_MATCH_MP weak_exec_to_n thm)]) >>
+PAT_ASSUM ``weak_model m`` (fn thm => fs [GSYM (HO_MATCH_MP weak_exec_exists thm)]) >>
+irule weak_inter >>
+fs [] >>
+qexistsl_tac [`ls1`, `ms'''`] >>
+fs [] >>
+subgoal `ms' <> ms''` >- (
+QSPECL_X_ASSUM ``!n_l'.
+          n_l' < n_l ==> weak_exec_n m ms (ls1 UNION ls2) n_l' <> SOME ms'`` [`SUC n_l'`] >>
+ gs []
+) >>
+metis_tac [weak_union_pc]
+QED
+
+Theorem weak_inter_exec:
+ !m.
+ weak_model m ==>
+ !ms ls1 ls2 n_l ms' ms''.
+ m.weak ms ls2 ms' ==>
+ DISJOINT ls1 ls2 ==>
+ (OLEAST n. weak_exec_n m ms (ls1 UNION ls2) n = SOME ms') = SOME n_l ==>
+ SING (\n. n < n_l /\ weak_exec_n m ms (ls1 UNION ls2) n = SOME ms'') ==>
+ m.weak ms'' ls2 ms'
+Proof
+rpt strip_tac >>
+PAT_ASSUM ``weak_model m`` (fn thm => fs [HO_MATCH_MP weak_exec_exists thm]) >>
+PAT_ASSUM ``weak_model m`` (fn thm => fs [HO_MATCH_MP weak_exec_to_n thm]) >>
+irule weak_exec_n_inter >>
+fs [pred_setTheory.SING_DEF, whileTheory.OLEAST_EQ_SOME] >>
+fs [GSYM pred_setTheory.UNIQUE_MEMBER_SING] >>
+qexistsl_tac [`ls1`, `ms`, `n_l`, `x`] >>
+fs [] >>
+rpt strip_tac >>
+QSPECL_X_ASSUM  ``!y. y < n_l /\ weak_exec_n m ms (ls1 UNION ls2) y = SOME ms'' ==> x = y`` [`n_l'`] >>
+subgoal `n_l' < n_l` >- (
+ gs []
+) >>
+fs []
+QED
+
+Theorem weak_exec_n_OLEAST_equiv:
+ !m. weak_model m ==>
+ !s ls s'.
+  (OLEAST n_l. n_l > 0 /\ weak_exec_n m s ls n_l = SOME s') = SOME 1 ==>
+  m.weak s ls s'
+Proof
+rpt strip_tac >>
+fs [whileTheory.OLEAST_EQ_SOME] >>
+PAT_ASSUM ``weak_model m`` (fn thm => fs [GSYM (HO_MATCH_MP weak_exec_to_n thm)]) >>
+PAT_ASSUM ``weak_model m`` (fn thm => fs [GSYM (HO_MATCH_MP weak_exec_exists thm)])
+QED
+
+(* Continuing weak_exec_n at s'', intermediately between s and s'' *)
+Theorem weak_exec_n_OLEAST_inter:
+ !m. weak_model m ==>
+ !s s' s'' ls n' n'' n_l.
+ (OLEAST n'. FUNPOW_OPT m.trs n' s = SOME s') = SOME n' ==>
+ (OLEAST n''. n'' > 0 /\ FUNPOW_OPT m.trs n'' s = SOME s'') = SOME n'' ==>
+ n' > n'' ==>
+ (OLEAST n_l. n_l > 0 /\ weak_exec_n m s ls n_l = SOME s'') = SOME 1 ==>
+ (OLEAST n_l. weak_exec_n m s'' ls n_l = SOME s') = SOME n_l ==>
+ (OLEAST n_l. weak_exec_n m s ls n_l = SOME s') = SOME (n_l + 1)
+Proof
+rpt strip_tac >>
+simp [whileTheory.OLEAST_EQ_SOME] >>
+conj_tac >| [
+ metis_tac [arithmeticTheory.ADD1, weak_exec_incr_first, weak_exec_n_OLEAST_equiv],
+
+ fs [whileTheory.OLEAST_EQ_SOME] >>
+ subgoal `s <> s'` >- (
+  QSPECL_X_ASSUM ``!n''. n'' < n' ==> FUNPOW_OPT m.trs n'' s <> SOME s'`` [`0`] >>
+  subgoal `0 < n'` >- (
+   fs []
+  ) >>
+  gs [FUNPOW_OPT_compute]
+ ) >>
+ subgoal `s'' <> s'` >- (
+  QSPECL_X_ASSUM ``!n''. n'' < n' ==> FUNPOW_OPT m.trs n'' s <> SOME s'`` [`n''`] >>
+  gs []
+ ) >>
+ subgoal `n_l > 0` >- (
+  Cases_on `n_l = 0` >- (
+   fs [weak_exec_n_def, FUNPOW_OPT_compute]
+  ) >>
+  fs []
+ ) >>
+ `weak_exec_n m s ls 1 <> SOME s' /\ !n_l'. n_l' < n_l ==> weak_exec_n m s'' ls n_l' <> SOME s'` suffices_by (
+  rpt strip_tac >>
+  fs [] >>
+  QSPECL_X_ASSUM ``!n_l'. n_l' < n_l ==> weak_exec_n m s'' ls n_l' <> SOME s'`` [`n_l' - 1`] >>
+  gs [] >>
+  subgoal `n_l' >= 1` >- (
+   Cases_on `n_l' = 0` >- (
+    fs [weak_exec_n_def, FUNPOW_OPT_compute]
+   ) >>
+   fs []
+  ) >>
+  metis_tac [weak_exec_n_split2]
+ ) >>
+ QSPECL_X_ASSUM ``!n''. n'' < n' ==> FUNPOW_OPT m.trs n'' s <> SOME s'`` [`n''`] >>
+ gs [] 
+]
+QED
+
+Theorem weak_exec_1_superset_lemma:
+ !m.
+ weak_model m ==>
+ !ls1 ls2 s'.
+ !n n'. n' <= n ==>
+        n' >= 1 ==>
+        !s. m.weak s ls1 s' /\ ((OLEAST n'. FUNPOW_OPT m.trs n' s = SOME s') = SOME n') ==>
+        s <> s' ==>
+        ls1 SUBSET ls2 ==>
+        ?n_l. n_l >= 1 /\ (OLEAST n_l. weak_exec_n m s ls2 n_l = SOME s') = SOME n_l
+Proof
+ntac 5 strip_tac >>
+Induct_on `n` >- (
+ fs []
+) >>
+rpt strip_tac >>
+Cases_on `n' < SUC n` >- (
+ QSPECL_X_ASSUM ``!n'. _`` [`n'`] >>
+ gs []
+) >>
+subgoal `n' = SUC n` >- (
+ fs [] 
+) >>
+Cases_on `n = 0` >- (
+ gs [] >>
+ subgoal `n' = 1` >- (
+  fs [] 
+ ) >>
+ fs [whileTheory.OLEAST_EQ_SOME] >>
+ qexists_tac `1` >>
+ fs [] >>
+ conj_tac >| [
+  PAT_ASSUM ``weak_model m`` (fn thm => fs [GSYM (HO_MATCH_MP weak_exec_to_n thm)]) >>
+  PAT_ASSUM ``weak_model m`` (fn thm => fs [GSYM (HO_MATCH_MP weak_exec_exists thm)]) >>
+  PAT_ASSUM ``weak_model m`` (fn thm => fs [HO_MATCH_MP (fst $ EQ_IMP_RULE (Q.SPEC `m` weak_model_def)) thm]) >>
+  qexists_tac `1` >>
+  fs [] >>
+  metis_tac [weak_pc_in_thm, pred_setTheory.SUBSET_THM],
+
+  rpt strip_tac >>
+  subgoal `n_l' = 0` >- (
+   fs [] 
+  ) >>
+  fs [weak_exec_n_def, FUNPOW_OPT_compute]
+ ]
+) >>
+(* 1. There exists a state s'' which we go to with weak-ls2 from s. (weak_superset_thm should suffice)
+ * s'' is reached with more trs than s': contradiction.
+ * s'' is reached with same amount of trs as s': s'' is s', proof completed
+ * with witness n_l''.
+ * s'' is reached with fewer trs than s': use induction hypothesis specialised for s'', then add
+ * numbers of weak-ls2 transitions together for the witness. *)
+subgoal `?s''. (OLEAST n_l''. n_l'' > 0 /\ weak_exec_n m s ls2 n_l'' = SOME s'') = SOME 1` >- (
+ subgoal `?ms''. m.weak s (ls1 UNION ls2) ms''` >- (
+  metis_tac [weak_superset_thm]
+ ) >>
+ qexistsl_tac [`ms''`] >>
+ fs [whileTheory.OLEAST_EQ_SOME] >>
+ metis_tac [weak_subset, weak_exec_to_n, weak_exec_exists]
+) >>
+subgoal `?n''. (OLEAST n''. n'' > 0 /\ FUNPOW_OPT m.trs n'' s = SOME s'') = SOME n''` >- (
+ (* Since s'' is reached by non-zero weak transitions, there must be a (least) non-zero number of trs
+  * that reaches it *)
+ fs [whileTheory.OLEAST_EQ_SOME] >>
+ PAT_ASSUM ``weak_model m`` (fn thm => fs [GSYM (HO_MATCH_MP weak_exec_to_n thm)]) >>
+ PAT_ASSUM ``weak_model m`` (fn thm => fs [GSYM (HO_MATCH_MP weak_exec_exists thm)]) >>
+ PAT_ASSUM ``weak_model m`` (fn thm => fs [HO_MATCH_MP (fst $ EQ_IMP_RULE (Q.SPEC `m` weak_model_def)) thm]) >>
+ qexists_tac `n'''` >>
+ fs [] >>
+ rpt strip_tac >>
+ QSPECL_X_ASSUM ``!n'.
+          n' < n'3' /\ n' > 0 ==>
+          ?ms''. FUNPOW_OPT m.trs n' s = SOME ms'' /\ m.pc ms'' NOTIN ls2`` [`n''''`] >>
+ gs []
+) >>
+(* s'' is reached with more trs than s': contradiction, s' would have been crossed *)
+Cases_on `n'' > n'` >- (
+ fs [whileTheory.OLEAST_EQ_SOME] >>
+ subgoal `m.weak s ls2 s''` >- (
+  metis_tac [weak_exec_to_n, weak_exec_exists]
+ ) >>
+ PAT_ASSUM ``weak_model m`` (fn thm => fs [HO_MATCH_MP (fst $ EQ_IMP_RULE (Q.SPEC `m` weak_model_def)) thm]) >>
+ (* TODO: Make some kind of lemma here? *)
+ Q.SUBGOAL_THEN `n'4' = n''` (fn thm => fs [thm]) >- (
+  Cases_on `n'' < n'4'` >- (
+   QSPECL_X_ASSUM ``!n'.
+          n' < n'4' /\ n' > 0 ==>
+          ?ms''. FUNPOW_OPT m.trs n' s = SOME ms'' /\ m.pc ms'' NOTIN ls2`` [`n''`] >>
+   gs []
+  ) >>
+  Cases_on `n'' > n'4'` >- (
+   QSPECL_X_ASSUM ``!n'3'.
+          n'3' < n'' ==> FUNPOW_OPT m.trs n'3' s = SOME s'' ==> ~(n'3' > 0)`` [`n''''`] >>
+   gs []
+  ) >>
+  fs []
+ ) >>
+ (* TODO: Make some kind of lemma here? *)
+ Q.SUBGOAL_THEN `n'3' = n'` (fn thm => fs [thm]) >- (
+  Cases_on `n' < n'3'` >- (
+   QSPECL_X_ASSUM ``!n'.
+          n' < n'3' /\ n' > 0 ==>
+          ?ms''. FUNPOW_OPT m.trs n' s = SOME ms'' /\ m.pc ms'' NOTIN ls1`` [`n'`] >>
+   gs []
+  ) >>
+  Cases_on `n' > n'3'` >- (
+   QSPECL_X_ASSUM ``!n'.
+          n' < n'3' /\ n' > 0 ==>
+          ?ms''. FUNPOW_OPT m.trs n' s = SOME ms'' /\ m.pc ms'' NOTIN ls1`` [`n'''`] >>
+   gs []
+  ) >>
+  fs []
+ ) >>
+ QSPECL_X_ASSUM ``!n'.
+          n' < n'' /\ n' > 0 ==>
+          ?ms''. FUNPOW_OPT m.trs n' s = SOME ms'' /\ m.pc ms'' NOTIN ls2`` [`n'`] >>
+ gs [] >>
+ metis_tac [pred_setTheory.SUBSET_THM]
+) >>
+Cases_on `n'' = n'` >- (
+ qexists_tac `1` >>
+ subgoal `s'' = s'` >- (
+  fs [whileTheory.OLEAST_EQ_SOME]
+ ) >>
+ fs [whileTheory.OLEAST_EQ_SOME] >>
+ rpt strip_tac >>
+ subgoal `n_l = 0` >- (
+  fs []
+ ) >>
+ fs [weak_exec_n_def, FUNPOW_OPT_compute]
+) >>
+subgoal `n'' < n'` >- (
+ fs []
+) >>
+QSPECL_X_ASSUM ``!n'. _`` [`n' - n''`] >>
+rfs [] >>
+subgoal `n' <= n + n''` >- (
+ gs [whileTheory.OLEAST_EQ_SOME]
+) >>
+fs [] >>
+QSPECL_X_ASSUM ``!s'''. _`` [`s''`] >>
+(* Should be possible to prove with some inter theorem... *)
+subgoal `m.weak s'' ls1 s'` >- (
+ (* Next state in s'' is s'... *)
+ PAT_ASSUM ``weak_model m`` (fn thm => simp [HO_MATCH_MP (fst $ EQ_IMP_RULE (Q.SPEC `m` weak_model_def)) thm]) >>
+ qexists_tac `n' - n''` >>
+ fs [] >>
+ rpt conj_tac >| [
+  irule FUNPOW_OPT_split >>
+  qexistsl_tac [`n'`, `s`] >>
+  fs [whileTheory.OLEAST_EQ_SOME],
+
+  metis_tac [weak_pc_in_thm],
+
+  rpt strip_tac >>
+  fs [whileTheory.OLEAST_EQ_SOME] >>
+  PAT_ASSUM ``weak_model m`` (fn thm => fs [HO_MATCH_MP (fst $ EQ_IMP_RULE (Q.SPEC `m` weak_model_def)) thm]) >>
+  (* TODO: Make some kind of lemma here? *)
+  subgoal `n'''' = n'` >- (
+   Cases_on `n' < n'4'` >- (
+    QSPECL_X_ASSUM ``!n'.
+           n' < n'4' /\ n' > 0 ==>
+           ?ms''. FUNPOW_OPT m.trs n' s = SOME ms'' /\ m.pc ms'' NOTIN ls1`` [`n'`] >>
+    gs []
+   ) >>
+   Cases_on `n' > n'4'` >- (
+    QSPECL_X_ASSUM ``!n''. n'' < n' ==> FUNPOW_OPT m.trs n'' s <> SOME s'`` [`n''''`] >>
+    gs []
+   ) >>
+   fs []
+  ) >>
+  gs [] >>
+  QSPECL_X_ASSUM ``!n'5'.
+          n'5' < n' /\ n'5' > 0 ==>
+          ?ms''. FUNPOW_OPT m.trs n'5' s = SOME ms'' /\ m.pc ms'' NOTIN ls1`` [`n''' + n''`] >>
+  gs [] >>
+  qexists_tac `ms''` >>
+  fs [] >>
+  irule FUNPOW_OPT_split >>
+  qexistsl_tac [`n'' + n'3'`, `s`] >>
+  fs []
+ ]
+) >>
+fs [] >>
+subgoal `(OLEAST n'. FUNPOW_OPT m.trs n' s'' = SOME s') = SOME (n' - n'')` >- (
+ fs [whileTheory.OLEAST_EQ_SOME] >>
+ conj_tac >| [
+  irule FUNPOW_OPT_split >>
+  qexistsl_tac [`n'`, `s`] >>
+  fs [],
+
+  rpt strip_tac >>
+  QSPECL_X_ASSUM ``!n''. n'' < n' ==> FUNPOW_OPT m.trs n'' s <> SOME s'`` [`n'' + n'''`] >>
+  gs [] >>
+  metis_tac [FUNPOW_OPT_ADD_thm, arithmeticTheory.ADD_COMM]
+ ]
+) >>
+fs [] >>
+subgoal `s'' <> s'` >- (
+ (* Since s'' NOTIN ls1, while s' IN ls1 *)
+ PAT_ASSUM ``weak_model m`` (fn thm => fs [HO_MATCH_MP (fst $ EQ_IMP_RULE (Q.SPEC `m` weak_model_def)) thm]) >>
+ (* TODO: Make some kind of lemma here? *)
+ Q.SUBGOAL_THEN `n'3' = n'` (fn thm => fs [thm]) >- (
+  Cases_on `n' < n'3'` >- (
+   QSPECL_X_ASSUM ``!n'.
+          n' < n'3' /\ n' > 0 ==>
+          ?ms''. FUNPOW_OPT m.trs n' s = SOME ms'' /\ m.pc ms'' NOTIN ls1`` [`n'`] >>
+   gs [whileTheory.OLEAST_EQ_SOME]
+  ) >>
+  Cases_on `n' > n'3'` >- (
+   gs [whileTheory.OLEAST_EQ_SOME]
+  ) >>
+  fs []
+ ) >>
+ QSPECL_X_ASSUM ``!n'5'.
+          n'5' < n' /\ n'5' > 0 ==>
+          ?ms''. FUNPOW_OPT m.trs n'5' s = SOME ms'' /\ m.pc ms'' NOTIN ls1`` [`n''`] >>
+ gs [whileTheory.OLEAST_EQ_SOME] >>
+ strip_tac >>
+ fs []
+) >>
+fs [] >>
+qexists_tac `1 + n_l` >>
+fs [] >>
+irule weak_exec_n_OLEAST_inter >>
+fs [] >>
+qexistsl_tac [`n''`, `s''`] >>
+fs []
+QED
+
+(* TODO: Generalise this *)
+(* TODO: Change weak_exec_n 1 to weak? *)
+Theorem weak_exec_1_superset:
+ !m.
+ weak_model m ==>
+ !ms ls1 ls2 ms'.
+ weak_exec_n m ms ls1 1 = SOME ms' ==>
+ ms <> ms' ==>
+ ls1 SUBSET ls2 ==>
+ ?n. n >= 1 /\ (OLEAST n. weak_exec_n m ms ls2 n = SOME ms') = SOME n
+Proof
+rpt strip_tac >>
+PAT_ASSUM ``weak_model m`` (fn thm => fs [GSYM (HO_MATCH_MP weak_exec_to_n thm)]) >>
+PAT_ASSUM ``weak_model m`` (fn thm => fs [GSYM (HO_MATCH_MP weak_exec_exists thm)]) >>
+subgoal `?n'. n' > 0 /\ (OLEAST n'. FUNPOW_OPT m.trs n' ms = SOME ms') = SOME n'` >- (
+ (* Since weak goes from ms to ms', there must be a least number of primitive transitions such that
+  * ms goes to ms' *)
+ metis_tac [weak_least_trs]
+) >>
+irule weak_exec_1_superset_lemma >>
+fs [] >>
+rpt strip_tac >| [
+ qexists_tac `n'` >>
+ fs [],
+
+ metis_tac []
+]
+QED
+
+(* TODO: Strengthen conclusion to state either ms'' is ms', or pc is in ls2? *)
+Theorem weak_exec_exists_superset:
+ !m.
+ weak_model m ==>
+ !ms ls1 ls2 ms'. 
+ m.weak ms ls1 ms' ==>
+ ?ms''. weak_exec m (ls1 UNION ls2) ms = SOME ms''
+Proof
+rpt strip_tac >>
+fs [weak_exec_def, weak_nonempty] >>
+metis_tac [weak_superset_thm]
+QED
+
+(* Note: ms <> ms' used to avoid proving case where least n is zero *)
+Theorem weak_exec_n_exists_superset:
+ !m.
+ weak_model m ==>
+ !ms ls1 ls2 ms'. 
+ m.weak ms ls1 ms' ==>
+ ms <> ms' ==>
+ ?n. (OLEAST n. weak_exec_n m ms (ls1 UNION ls2) n = SOME ms') = SOME n
+Proof
+rpt strip_tac >>
+fs [whileTheory.OLEAST_EQ_SOME] >>
+subgoal `weak_exec_n m ms ls1 1 = SOME ms'` >- (
+ PAT_ASSUM ``weak_model m`` (fn thm => fs [HO_MATCH_MP weak_exec_exists thm]) >>
+ PAT_ASSUM ``weak_model m`` (fn thm => fs [HO_MATCH_MP weak_exec_to_n thm])
+) >>
+imp_res_tac weak_exec_1_superset >>
+QSPECL_X_ASSUM ``!ls2. _`` [`ls1 UNION ls2`] >>
+fs [] >>
+qexists_tac `n` >>
+fs [whileTheory.OLEAST_EQ_SOME]
+QED
+
+Theorem weak_exec_least_nonzero:
+ !m.
+ weak_model m ==>
+ !ms ls ms' n_l.
+ (OLEAST n. weak_exec_n m ms ls n = SOME ms') = SOME n_l ==>
+ ms <> ms' ==>
+ n_l > 0
+Proof
+rpt strip_tac >>
+Cases_on `n_l` >> (
+ fs []
+) >>
+fs [whileTheory.OLEAST_EQ_SOME, weak_exec_n_def, FUNPOW_OPT_def]
+QED
+
+Theorem weak_exec_sing_least_less:
+ !m.
+ weak_model m ==>
+ !ms ls ms' n_l.
+ SING (\n. n < n_l /\ weak_exec_n m ms ls n = SOME ms') ==>
+ ?n_l'. (OLEAST n. weak_exec_n m ms ls n = SOME ms') = SOME n_l' /\ n_l' < n_l
+Proof
+rpt strip_tac >>
+fs [pred_setTheory.SING_DEF, whileTheory.OLEAST_EQ_SOME] >>
+qexists_tac `x` >>
+rpt strip_tac >> (
+ fs [GSYM pred_setTheory.UNIQUE_MEMBER_SING]
+) >>
+QSPECL_X_ASSUM ``!y. y < n_l /\ weak_exec_n m ms ls y = SOME ms' ==> x = y`` [`n`] >>
+gs []
+QED
+
+
+(* TODO: Technically, this doesn't need OLEAST for the encounter of ms' *)
+Theorem weak_exec_incr_least:
+ !m.
+ weak_model m ==>
+ !ms ls ms' ms_e n_l n_l' ms''.
+ (OLEAST n. weak_exec_n m ms ls n = SOME ms_e) = SOME n_l ==>
+ ms'' <> ms_e ==>
+ (OLEAST n. weak_exec_n m ms ls n = SOME ms') = SOME n_l' ==>
+ m.weak ms' ls ms'' ==>
+ SING (\n. n < n_l /\ weak_exec_n m ms ls n = SOME ms'') ==>
+ n_l' < n_l ==>
+ (OLEAST n. weak_exec_n m ms ls n = SOME ms'') = SOME (SUC n_l')
+Proof
+rpt strip_tac >>
+imp_res_tac weak_exec_incr_last >>
+fs [whileTheory.OLEAST_EQ_SOME] >>
+rpt strip_tac >>
+subgoal `SUC n_l' < n_l` >- (
+ Cases_on `SUC n_l' = n_l` >- (
+  fs []
+ ) >>
+ fs []
+) >>
+fs [pred_setTheory.SING_DEF] >>
+fs [GSYM pred_setTheory.UNIQUE_MEMBER_SING] >>
+QSPECL_ASSUM ``!y. y < n_l /\ weak_exec_n m ms ls y = SOME ms'' ==> x = y`` [`SUC n_l'`] >>
+QSPECL_X_ASSUM ``!y. y < n_l /\ weak_exec_n m ms ls y = SOME ms'' ==> x = y`` [`n`] >>
+gs []
+(* Due to SING (\n. n < n_l /\ weak_exec_n m ms ls n = SOME ms''),
+ * both weak_exec_n m ms ls (SUC n_l') and weak_exec_n m ms ls n
+ * can't lead to ms''. NOTE: Requires SUC n_l' < n_l *)
+(* OK: If ms' was first encountered at n_l' weak iterations to ls, and
+ * if one additional weak transition to ls goes to ms'', then if
+ * ms'' is uniquely encountered before n_l weak transitions to ls and n_l
+ * is greater than n_l', then SUC n_l' must be the least number of weak transitions
+ * needed to reach ms'' *)
+QED
+
+Theorem weak_exec_uniqueness:
+ !m.
+ weak_model m ==>
+ !ms ls ms' ms'' ms''' n_l n_l'. 
+ (OLEAST n. weak_exec_n m ms ls n = SOME ms') = SOME n_l ==>
+ (OLEAST n. weak_exec_n m ms ls n = SOME ms'') = SOME n_l' ==>
+ n_l' < n_l ==>
+ m.weak ms'' ls ms''' ==>
+ ms''' <> ms' ==>
+ SING (\n_l''. n_l'' < n_l /\ weak_exec_n m ms ls n_l'' = SOME ms''')
+Proof
+rpt strip_tac >>
+subgoal `weak_exec_n m ms ls (n_l' + 1) = SOME ms'3'` >- (
+ irule weak_exec_n_add >>
+ fs [whileTheory.OLEAST_EQ_SOME] >>
+ metis_tac [weak_exec_exists, weak_exec_to_n]
+) >>
+(* Suppose there exists some earlier encounter of ms''' *)
+Cases_on `?n_l''. n_l'' < (n_l' + 1) /\ weak_exec_n m ms ls n_l'' = SOME ms'''` >- (
+ fs [whileTheory.OLEAST_EQ_SOME] >>
+ subgoal `weak_exec_n m ms''' ls (n_l - (n_l' + 1)) = SOME ms'` >- (
+  irule weak_exec_n_split2 >>
+  fs [] >>
+  qexists_tac `ms` >>
+  fs []
+ ) >>
+ subgoal `weak_exec_n m ms ls (n_l'' + (n_l - (n_l' + 1))) = SOME ms'` >- (
+  irule weak_exec_n_add >>
+  fs [] >>
+  qexists_tac `ms'3'` >>
+  fs []
+ ) >>
+ QSPECL_ASSUM ``!n. n < n_l ==> weak_exec_n m ms ls n <> SOME ms'`` [`(n_l'' + (n_l - (n_l' + 1)))`] >>
+ gs []
+) >>
+fs [] >>
+(* If there were no earlier encounter of ms''', then the first encounter was at n_l' + 1 *)
+subgoal `(OLEAST n_l. weak_exec_n m ms ls n_l = SOME ms''') = SOME (n_l' + 1)` >- (
+ fs [whileTheory.OLEAST_EQ_SOME] >>
+ metis_tac []
+) >>
+
+(* Suppose there exists some later encounter of ms''' *)
+Cases_on `?n_l''. n_l'' > (n_l' + 1) /\ n_l'' < n_l /\ weak_exec_n m ms ls n_l'' = SOME ms'''` >- (
+ fs [] >>
+ subgoal `(OLEAST n_l. weak_exec_n m ms''' ls n_l = SOME ms') = SOME (n_l - (n_l' + 1))` >- (
+  fs [whileTheory.OLEAST_EQ_SOME] >>
+  rpt strip_tac >| [
+   irule weak_exec_n_split2 >>
+   fs [] >>
+   qexists_tac `ms` >>
+   fs [],
+
+   (* TODO: Prove the OLEAST part... *)
+   subgoal `weak_exec_n m ms ls ((n_l' + 1) + n_l'3') <> SOME ms'` >- (
+    QSPECL_ASSUM ``!n. n < n_l ==> weak_exec_n m ms ls n <> SOME ms'`` [`(n_l' + 1) + n_l'3'`] >>
+    gs []
+   ) >>
+   subgoal `weak_exec_n m ms ls ((n_l' + 1) + n_l'3') = SOME ms'` >- (
+    irule weak_exec_n_add >>
+    fs []
+   )
+  ]
+ ) >>
+ subgoal `weak_exec_n m ms''' ls (n_l'' - (n_l' + 1)) = SOME ms'''` >- (
+  irule weak_exec_n_split2 >>
+  fs [] >>
+  qexists_tac `ms` >>
+  fs []
+ ) >>
+ (* By weak_exec_n_cycle *)
+ subgoal `(n_l - (n_l' + 1)) < (n_l'' - (n_l' + 1))` >- (
+  irule weak_exec_n_cycle >>
+  fs [] >>
+  qexistsl_tac [`ls`, `m`, `ms'''`, `ms'`] >>
+  gs [whileTheory.OLEAST_EQ_SOME]
+ ) >>
+ gs []
+) >>
+fs [] >>
+gs [pred_setTheory.SING_DEF, GSYM pred_setTheory.UNIQUE_MEMBER_SING] >>
+qexists_tac `n_l' + 1` >>
+rpt strip_tac >| [
+ Cases_on `n_l' + 1 = n_l` >- (
+  gvs [whileTheory.OLEAST_EQ_SOME]
+ ) >>
+ gs [],
+
+ irule weak_exec_n_add >>
+ fs [] >>
+ qexists_tac `ms''` >>
+ fs [whileTheory.OLEAST_EQ_SOME] >>
+ metis_tac [weak_exec_exists, weak_exec_to_n],
+
+ res_tac >>
+ gs [arithmeticTheory.EQ_LESS_EQ, arithmeticTheory.NOT_LESS]
+]
+QED
+
+Theorem weak_exec_unique_start:
+ !m.
+ weak_model m ==>
+ !ms ls ms' n_l. 
+ (OLEAST n. weak_exec_n m ms ls n = SOME ms') = SOME n_l ==>
+ ms <> ms' ==>
+ SING (\n_l'. n_l' < n_l /\ weak_exec_n m ms ls n_l' = SOME ms)
+Proof
+rpt strip_tac >>
+gs [pred_setTheory.SING_DEF, GSYM pred_setTheory.UNIQUE_MEMBER_SING] >>
+qexists_tac `0` >>
+rpt strip_tac >| [
+ Cases_on `n_l = 0` >> (
+  fs [weak_exec_n_def, FUNPOW_OPT_compute, whileTheory.OLEAST_EQ_SOME]
+ ),
+
+ fs [weak_exec_n_def, FUNPOW_OPT_compute],
+
+ Cases_on `y > 0` >- (
+  imp_res_tac weak_exec_n_cycle >>
+  fs []
+ ) >>
+ fs []
+]
+QED
+
+(* Uses the fact that exit labels are disjoint from loop point to know that
+ * we have not yet exited the loop after another weak transition, i.e. the
+ * number of loops is still less than n_l *)
+Theorem weak_exec_less_incr_superset:
+ !m.
+ weak_model m ==>
+ !ms ls1 ls2 ms' ms'' ms''' n_l n_l'.
+ DISJOINT ls1 ls2 ==>
+ (OLEAST n. weak_exec_n m ms (ls1 UNION ls2) n = SOME ms') = SOME n_l ==>
+ m.pc ms' IN ls2 ==>
+ (OLEAST n. weak_exec_n m ms (ls1 UNION ls2) n = SOME ms'') = SOME n_l' ==>
+ n_l' < n_l ==>
+ m.weak ms'' (ls1 UNION ls2) ms''' ==>
+ m.pc ms''' NOTIN ls2 ==>
+ SUC n_l' < n_l
+Proof
+rpt strip_tac >>
+Cases_on `SUC n_l' = n_l` >- (
+ subgoal `ms''' = ms'` >- (
+  subgoal `weak_exec_n m ms (ls1 UNION ls2) (SUC n_l') = SOME ms'''` >- (
+   metis_tac [weak_exec_incr_last]
+  ) >>
+  gs [whileTheory.OLEAST_EQ_SOME]
+ ) >>
+ fs []
+) >>
+fs []
 QED
 
 
