src/aux/bir_auxiliaryScript.sml
@@ -199,6 +199,39 @@ SIMP_TAC arith_ss [rich_listTheory.SEG_TAKE_DROP] >>
 REPEAT STRIP_TAC >>
 ASM_SIMP_TAC list_ss [rich_listTheory.DROP_EL_CONS, arithmeticTheory.ADD1]);
 
+Theorem INDEX_FIND_SUFFIX:
+!P n i x_list x.
+i < n ==>
+INDEX_FIND 0 P x_list = SOME (PRE n, x) ==>
+INDEX_FIND 0 P (DROP i x_list) = SOME (PRE (n - i), x)
+Proof
+rpt strip_tac >>
+fs [INDEX_FIND_EQ_SOME_0] >>
+rpt strip_tac >| [
+ subgoal `EL (PRE (n - i)) (DROP i x_list) = EL ((PRE (n - i)) + i) x_list` >- (
+  irule listTheory.EL_DROP >>
+  fs []
+ ) >>
+ fs [] >>
+ `i + PRE (n - i) = PRE n` suffices_by (
+  rpt strip_tac >>
+  fs []
+ ) >>
+ fs [],
+
+ subgoal `j' + i < PRE n` >- (
+  fs [arithmeticTheory.LESS_MONO_ADD_EQ]
+ ) >>
+ Q.SUBGOAL_THEN `EL j' (DROP i x_list) = EL (j' + i) x_list` (fn thm => fs [thm]) >- (
+  irule listTheory.EL_DROP >>
+  fs []
+ ) >>
+ QSPECL_X_ASSUM ``!j'. j' < PRE n ==> ~P (EL j' x_list)`` [`i + j'`] >>
+ fs []
+]
+QED
+
+
 
 (* -------------------------------------------------------------------------- *)
 (* pred_set lemmata                                                           *)
@@ -371,6 +404,54 @@ BasicProvers.VAR_EQ_TAC >>
 `~(n1 < n2)` by METIS_TAC[] >>
 DECIDE_TAC);
 
+Theorem MEM_OLEAST:
+ !l x.
+ MEM x l ==>
+ ?i. (OLEAST i. oEL i l = SOME x) = SOME i
+Proof
+Induct >> (
+ fs [listTheory.MEM, listTheory.LENGTH]
+) >>
+rpt strip_tac >| [
+ qexists_tac `0` >>
+ fs [whileTheory.OLEAST_EQ_SOME, listTheory.oEL_THM],
+
+ qpat_assum `!x. _` (fn thm => imp_res_tac thm) >>
+ Cases_on `h = x` >- (
+  qexists_tac `0` >>
+  fs [whileTheory.OLEAST_EQ_SOME, listTheory.oEL_THM]
+ ) >>
+ qexists_tac `SUC i` >>
+ fs [whileTheory.OLEAST_EQ_SOME, listTheory.oEL_THM] >>
+ rpt strip_tac >>
+ Cases_on `i'` >- (
+  fs []
+ ) >>
+ QSPECL_X_ASSUM ``!i'. _`` [`n`] >>
+ gs []
+]
+QED
+
+Theorem FILTER_HD_OLEAST:
+ !P l l'.
+ FILTER P l = l' ==>
+ LENGTH l' > 0 ==>
+ ?i. (OLEAST i. oEL i l = SOME (HD l')) = SOME i
+Proof
+rpt strip_tac >>
+subgoal `MEM (HD l') l'` >- (
+ Cases_on `l'` >> (
+  fs [listTheory.NOT_NIL_EQ_LENGTH_NOT_0]
+ )
+) >>
+subgoal `MEM (HD l') l` >- (
+ metis_tac [listTheory.MEM_FILTER]
+) >>
+imp_res_tac MEM_OLEAST >>
+qexists_tac `i` >>
+fs []
+QED
+
 
 (* -------------------------------------------------------------------------- *)
 (* Optional Minimum                                                           *)
@@ -487,6 +568,11 @@ val OPT_CONS_REVERSE = store_thm ("OPT_CONS_REVERSE",
 Cases >> SIMP_TAC list_ss [OPT_CONS_REWRS]);
 
 
+(*******************)
+(*   FUNPOW_OPT    *)
+(*******************)
+(* TODO: How about renaming this to oFUNPOW? Similar to oEL, OLEAST, ... *)
+
 val FUNPOW_OPT_def = Define `
   FUNPOW_OPT (r : 'a -> 'a option) n x =
   FUNPOW (\x. option_CASE x NONE r) n (SOME x)`
@@ -574,6 +660,117 @@ Cases_on `FUNPOW_OPT step_fun n' s` >| [
   METIS_TAC []
 ]
 );
+
+Theorem FUNPOW_ASSOC:
+ !f m n x.
+ FUNPOW f m (FUNPOW f n x) = FUNPOW f n (FUNPOW f m x)
+Proof
+fs [GSYM arithmeticTheory.FUNPOW_ADD]
+QED
+
+Theorem FUNPOW_OPT_step:
+ !f n x x' x''.
+ FUNPOW_OPT f (SUC n) x = SOME x'' ==>
+ f x = SOME x' ==>
+ FUNPOW_OPT f n x' = SOME x''
+Proof
+rpt strip_tac >>
+fs [FUNPOW_OPT_REWRS]
+QED
+
+Theorem FUNPOW_OPT_PRE:
+ !f n x x' x''.
+ n > 0 ==>
+ FUNPOW_OPT f n x = SOME x' ==>
+ f x = SOME x'' ==>
+ FUNPOW_OPT f (PRE n) x'' = SOME x'
+Proof
+rpt strip_tac >>
+Cases_on `n` >> (
+ fs [FUNPOW_OPT_REWRS]
+)
+QED
+
+(* TODO: Use FUNPOW_OPT_next_n_NONE instead of this *)
+Theorem FUNPOW_OPT_ADD_NONE:
+ !f n n' ms ms'.
+ FUNPOW_OPT f n ms = SOME ms' ==>
+ FUNPOW_OPT f n' ms' = NONE ==> 
+ FUNPOW_OPT f (n'+n) ms = NONE
+Proof
+metis_tac [FUNPOW_OPT_def,
+           arithmeticTheory.FUNPOW_ADD]
+QED
+
+Theorem FUNPOW_OPT_INTER:
+ !f n n' ms ms' ms''.
+ FUNPOW_OPT f n ms = SOME ms' ==>
+ FUNPOW_OPT f (n'+n) ms = SOME ms'' ==>
+ FUNPOW_OPT f n' ms' = SOME ms''
+Proof
+metis_tac [FUNPOW_OPT_def,
+           arithmeticTheory.FUNPOW_ADD]
+QED
+
+Theorem FUNPOW_SUB:
+ !f m n x.
+ m > n ==>
+ FUNPOW f (m - n) (FUNPOW f n x) = FUNPOW f m x
+Proof
+fs [GSYM arithmeticTheory.FUNPOW_ADD]
+QED
+
+Theorem FUNPOW_OPT_split:
+!f n' n s s'' s'.
+n > n' ==>
+FUNPOW_OPT f n s = SOME s' ==>
+FUNPOW_OPT f (n - n') s = SOME s'' ==>
+FUNPOW_OPT f n' s'' = SOME s'
+Proof
+rpt strip_tac >>
+irule FUNPOW_OPT_INTER >>
+qexistsl_tac [`s`, `n - n'`] >>
+fs []
+QED
+
+Theorem FUNPOW_OPT_split2:
+!f n' n s s'' s'.
+n > n' ==>
+FUNPOW_OPT f n s = SOME s' ==>
+FUNPOW_OPT f n' s = SOME s'' ==>
+FUNPOW_OPT f (n - n') s'' = SOME s'
+Proof
+rpt strip_tac >>
+metis_tac [FUNPOW_SUB, FUNPOW_OPT_def, arithmeticTheory.FUNPOW_ADD]
+QED
+
+(* TODO: Relax the first OLEAST? *)
+Theorem FUNPOW_OPT_cycle:
+ !f s s' n n'.
+ (OLEAST n. n > 0 /\ FUNPOW_OPT f n s = SOME s) = SOME n ==>
+ s <> s' ==>
+ (OLEAST n'. FUNPOW_OPT f n' s = SOME s') = SOME n' ==>
+ n' < n
+Proof
+rpt strip_tac >>
+CCONTR_TAC >>
+Cases_on `n' = n` >- (
+ fs [whileTheory.OLEAST_EQ_SOME]
+) >>
+subgoal `n' > n` >- (
+ gs []
+) >>
+subgoal `FUNPOW_OPT f (n' - n) s = SOME s'` >- (
+ irule FUNPOW_OPT_split2 >>
+ fs [whileTheory.OLEAST_EQ_SOME] >>
+ qexists_tac `s` >>
+ fs []
+) >>
+fs [whileTheory.OLEAST_EQ_SOME] >>
+QSPECL_X_ASSUM ``!n''. n'' < n' ==> FUNPOW_OPT f n'' s <> SOME s'`` [`n' - n`] >>
+gs []
+QED
+
 
 (* -------------------------------------------------------------------------- *)
 (* lazy lists                                                                 *)
